#################################################################
#    Ontology to describe cases heard by the Judicial Committee 
#    of the Privy Council (JCPC)
#
#    Version 4
#    Created by ds-anon-test, 15 November 2017 (modified 2 February 2018)
#################################################################

@prefix owl: <http://www.w3.org/2002/07/owl#> .
@prefix rdf: <http://www.w3.org/1999/02/22-rdf-syntax-ns#> .
@prefix xml: <http://www.w3.org/XML/1998/namespace> .
@prefix xsd: <http://www.w3.org/2001/XMLSchema#> .
@prefix rdfs: <http://www.w3.org/2000/01/rdf-schema#> .
@prefix dc: <http://purl.org/dc/terms/> .
@prefix dul: <http://www.ontologydesignpatterns.org/ont/dul/DUL.owl#> .
@prefix foaf: <http://xmlns.com/foaf/0.1/> .
@prefix jcpc: <http://data.bl.uk/jcpc/ontology/> .
@prefix vcard: <http://www.w3.org/2006/vcard/ns#> .
@prefix wikidata: <http://www.wikidata.org/entity/> .
@prefix lkif-action: <http://www.estrellaproject.org/lkif-core/action.owl#> .
@base <http://data.bl.uk/jcpc/ontology/> .

### The below URI will not resolve until the full dataset is published.
<http://data.bl.uk/jcpc/ontology/> rdf:type owl:Ontology .

#################################################################
#    Object Properties
#################################################################

###  has Appellant
jcpc:hasAppellant rdf:type owl:ObjectProperty ;
                       rdfs:label "has Appellant"@en ;
                       rdfs:comment "Property of Appeal; refers to an Appellant who brought that Appeal to the JCPC"@en ;
                       owl:InverseOf jcpc:isAppellantOf ;
                       rdfs:range jcpc:Appellant .


###  is Appellant of
jcpc:isAppellantOf rdf:type owl:ObjectProperty ;
                       rdfs:label "is Appellant of"@en ;
                       rdfs:comment "Property of Appellant; refers to an Appeal brought to the JCPC by that Appellant"@en ;
                       owl:InverseOf jcpc:hasAppellant ;
                       rdfs:range wikidata:Q329777 .


###  has Intervenant
jcpc:hasIntervenant rdf:type owl:ObjectProperty ;
                       rdfs:label "has Intervenant"@en ;
                       rdfs:comment "Property of Appeal; refers to an Intervenant involved with that Appeal"@en ;
                       owl:InverseOf jcpc:isIntervenantOf ;
                       rdfs:range jcpc:Intervenant .


###  is Intervenant of
jcpc:isIntervenantOf rdf:type owl:ObjectProperty ;
                       rdfs:label "is Intervenant of"@en ;
                       rdfs:comment "Property of Intervenant; refers to an Appeal with which that Intervenant was involved"@en ;
                       owl:InverseOf jcpc:hasIntervenant ;
                       rdfs:range wikidata:Q329777 .


###  has Judgment
jcpc:hasJudgment rdf:type owl:ObjectProperty ;
                       rdfs:label "has Judgment"@en ;
                       rdfs:comment "Property of Appeal; refers to a Judgment resulting from that Appeal"@en ;
                       owl:InverseOf jcpc:isJudgmentOf ;
                       rdfs:range wikidata:Q327000 .


###  is Judgment of
jcpc:isJudgmentOf rdf:type owl:ObjectProperty ;
                       rdfs:label "is Judgment of"@en ;
                       rdfs:comment "Property of Judgment; refers to an Appeal which resulted in that Judgment"@en ;
                       owl:InverseOf jcpc:hasJudgment ;
                       rdfs:range wikidata:Q329777 .

                       
###  has Location
dul:hasLocation rdf:type owl:ObjectProperty ;
                       rdfs:label "has Location"@en ;
                       rdfs:comment "Property of Appeal; refers to the Location where that Appeal originated"@en ;
                       owl:InverseOf jcpc:isLocationOf ;
                       rdfs:range vcard:Location .


###  is Location of
dul:isLocationOf rdf:type owl:ObjectProperty ;
                       rdfs:label "is Location of"@en ;
                       rdfs:comment "Property of Location; refers to an Appeal originating from that Location"@en ;
                       owl:InverseOf jcpc:hasLocation ;
                       rdfs:range wikidata:Q329777 .

                       
###  has Respondent
jcpc:hasRespondent rdf:type owl:ObjectProperty ;
                       rdfs:label "has Respondent"@en ;
                       rdfs:comment "Property of Appeal; refers to a Respondent who responded to that Appeal"@en ;
                       owl:InverseOf jcpc:isRespondentOf ;
                       rdfs:range jcpc:Respondent .


###  is Respondent of
jcpc:isRespondentOf rdf:type owl:ObjectProperty ;
                       rdfs:label "is Respondent of"@en ;
                       rdfs:comment "Property of Respondent; refers to an Appeal to which that Respondent responded"@en ;
                       owl:InverseOf jcpc:hasRespondent ;
                       rdfs:range wikidata:Q329777 .


###  has Third Party
jcpc:hasThirdParty rdf:type owl:ObjectProperty ;
                       rdfs:label "has Third Party"@en ;
                       rdfs:comment "Property of Appeal; refers to a Third Party involved with that Appeal"@en ;
                       owl:InverseOf jcpc:isThirdPartyOf ;
                       rdfs:range jcpc:ThirdParty .


###  is ThirdParty of
jcpc:isThirdPartyOf rdf:type owl:ObjectProperty ;
                       rdfs:label "is Third Party of"@en ;
                       rdfs:comment "Property of Third Party; refers to an Appeal with which that Third Party was involved"@en ;
                       owl:InverseOf jcpc:hasThirdParty ;
                       rdfs:range wikidata:Q329777 .

###  originating Court
jcpc:originatingCourt rdf:type owl:ObjectProperty ;
                       rdfs:label "originating Court"@en ;
                       rdfs:comment "Property of Appeal; refers to the Court where that Appeal originated"@en ;
                       owl:InverseOf jcpc:originOf ;
                       rdfs:range wikidata:Q41487 .


###  origin of
jcpc:originOf rdf:type owl:ObjectProperty ;
                       rdfs:label "origin of"@en ;
                       rdfs:comment "Property of Court; refers to an Appeal originating from that Court"@en ;
                       owl:InverseOf jcpc:originatingCourt ;
                       rdfs:range wikidata:Q329777 .


###  relation
dc:relation rdf:type owl:ObjectProperty ;
						rdfs:label "related Judgment"@en ;
						rdfs:comment "Used as a property of Judgment to link to another Judgment known to relate to a similar (or the same) case"@en .


###  same As
owl:sameAs rdf:type owl:ObjectProperty ;
						rdfs:label "same as"@en ;
						rdfs:comment "Used to link an entity such as Location, Court, Appellant, Respondent, Intervenant and Third Party to a representation of that entity in an external source"@en .


#################################################################
#    Data properties
#################################################################

###  Appeal number
jcpc:appealNumber rdf:type owl:DatatypeProperty ;
						rdfs:label "Appeal number"@en ;
						rdfs:comment "The number assigned by the JCPC to an Appeal, included in the original documentation for the resulting Judgment(s)"@en ;
						rdfs:domain wikidata:Q329777 .


###  BAILII identifier
jcpc:bailiiIdentifier rdf:type owl:DatatypeProperty ;
						rdfs:label "BAILII identifier"@en ;
						rdfs:comment "The identifier assigned to a Judgment by the British and Irish Legal Information Institute (BAILII); used in citations"@en ;
						rdfs:domain wikidata:Q327000 .

						
###  city
vcard:locality rdf:type owl:DatatypeProperty ; 
						rdfs:label "city"@en ;
						rdfs:comment "The city where a Location is located"@en .


###  country-name
vcard:country-name rdf:type owl:DatatypeProperty ;
						rdfs:label "country"@en ;
						rdfs:comment "The country where a Location is located"@en .


###  date
dc:date rdf:type owl:DatatypeProperty ;
						rdfs:label "date"@en ;
						rdfs:comment "The date on which an Appeal or Judgment took place"@en .


###  description
dc:description rdf:type owl:DatatypeProperty ;
						rdfs:label "description"@en ;
						rdfs:comment "Descriptive text about a Judgment, Appellant, Respondent, Intervenant or Third Party"@en .


###  geographic coordinates [latitude, longitude]
vcard:geo rdf:type owl:DatatypeProperty ;
						rdfs:label "geographic coordinates"@en ;
						rdfs:comment "The geographic coordinates of a Location, in the format 'latitude, longitude'"@en .


###  has version
dc:hasVersion rdf:type owl:DatatypeProperty ;
						rdfs:label "has version"@en ;
						rdfs:comment "Used to provide the URL of the digitised documents for a Judgment"@en .


###  identifier
dc:identifier rdf:type owl:DatatypeProperty ;
						rdfs:label "identifier"@en ;
						rdfs:comment "Identification number assigned to an Appeal or Judgment, composed of the Appeal or Judgment year and number, separated by an underscore, e.g. 1860_1"@en .


###  Judgment number
jcpc:judgmentNumber rdf:type owl:DatatypeProperty ;
						rdfs:label "Judgment number"@en ;
						rdfs:comment "The number assigned by the JCPC to a Judgment, included in the original documentation for that Judgment and/or the original dataset from which this data was converted"@en ;
						rdfs:domain wikidata:Q327000 .


###  label
rdfs:label rdf:type owl:DatatypeProperty ;
						rdfs:label "label"@en ;
						rdfs:comment "Human-readable label for classes and properties"@en .


###  name
foaf:name rdf:type owl:DatatypeProperty ;
						rdfs:label "name"@en ;
						rdfs:comment "The name of an Appellant, Respondent, Intervenant, Third Party or Court"@en .


###  region
vcard:region rdf:type owl:DatatypeProperty ;
						rdfs:label "region"@en ;
						rdfs:comment "The region where a Location is located"@en .


###  title
dc:title rdf:type owl:DatatypeProperty ;
						rdfs:label "title"@en ;
						rdfs:comment "The title of an Appeal or Judgment, composed of the Appellant and Respondent names, separated by 'v.', followed by the Appeal or Judgment year"@en .


#################################################################
#    Classes
#################################################################

###  Appeal
wikidata:Q329777 rdf:type owl:Class ,
						[ rdf:type owl:Restriction ;
        					owl:onProperty jcpc:appealNumber ;
        					owl:maxCardinality 1
     					] ,
						[ rdf:type owl:Restriction ;
        					owl:onProperty dc:date ;
        					owl:maxCardinality 1
     					] ,
     					[ rdf:type owl:Restriction ;
        					owl:onProperty dc:identifier ;
        					owl:maxCardinality 1
     					] ,
						[ rdf:type owl:Restriction ;
        					owl:onProperty jcpc:originatingCourt ;
        					owl:maxCardinality 1
     					] ,
     					[ rdf:type owl:Restriction ;
        					owl:onProperty dc:title ;
        					owl:cardinality 1
     					] ;
						rdfs:label "Appeal"@en ;
						rdfs:comment "Wikidata definition: 'process for reviewing and changing court decisions'"@en .


###  Appellant
jcpc:Appellant rdfs:subClassOf lkif-action:Agent ,
    					[ rdf:type owl:Restriction ;
        					owl:onProperty jcpc:isAppellantOf ;
        					owl:allValuesFrom wikidata:Q329777
     					] ,
     					[ rdf:type owl:Restriction ;
        					owl:onProperty dc:description ;
        					owl:maxCardinality 1
     					] ,
     					[ rdf:type owl:Restriction ;
        					owl:onProperty foaf:name ;
        					owl:cardinality 1
     					] ;
     					rdfs:label "Appellant"@en ;
						rdfs:comment "Organisation or person (including those acting under the title of their official role) appealing to the JCPC"@en .


###  Court
wikidata:Q41487 rdf:type owl:Class ,
     					[ rdf:type owl:Restriction ;
        					owl:onProperty foaf:name ;
        					owl:cardinality 1
     					] ;
						rdfs:label "Court"@en ;
						rdfs:comment "Wikidata definition: 'judicial institution with the authority to resolve legal disputes'"@en .


###  Intervenant
jcpc:Intervenant rdfs:subClassOf lkif-action:Agent ,
						[ rdf:type owl:Restriction ;
        					owl:onProperty jcpc:isIntervenantOf ;
        					owl:allValuesFrom wikidata:Q329777
     					] ,
     					[ rdf:type owl:Restriction ;
        					owl:onProperty dc:description ;
        					owl:maxCardinality 1
     					] ,
     					[ rdf:type owl:Restriction ;
        					owl:onProperty foaf:name ;
        					owl:cardinality 1
     					] ;
						rdfs:label "Intervenant"@en ;
						rdfs:comment "Organisation or person (including those acting under the title of their official role) who is not an Appellant or Respondent, but who appears in the case to defend any interests of theirs that might otherwise be compromised by the court's decision"@en .


###  Judgment [Wikidata: court decision]
wikidata:Q327000 rdf:type owl:Class ,
     					[ rdf:type owl:Restriction ;
        					owl:onProperty jcpc:bailiiIdentifier ;
        					owl:maxCardinality 1
     					] ,
     					[ rdf:type owl:Restriction ;
        					owl:onProperty dc:date ;
        					owl:maxCardinality 1
     					] ,
     					[ rdf:type owl:Restriction ;
        					owl:onProperty dc:description ;
        					owl:maxCardinality 1
     					] ,
     					[ rdf:type owl:Restriction ;
        					owl:onProperty dc:hasVersion ;
        					owl:maxCardinality 1
     					] ,
     					[ rdf:type owl:Restriction ;
        					owl:onProperty dc:identifier ;
        					owl:cardinality 1
     					] ,
     					[ rdf:type owl:Restriction ;
        					owl:onProperty jcpc:judgmentNumber ;
        					owl:cardinality 1
     					] ,
     					[ rdf:type owl:Restriction ;
        					owl:onProperty dc:title ;
        					owl:cardinality 1
     					] ;
						rdfs:label "Judgment"@en ;
						rdfs:comment "Wikidata definition: 'formal decision made by a court'"@en .


###  Location
vcard:Location rdf:type owl:Class ,
     					[ rdf:type owl:Restriction ;
        					owl:onProperty vcard:geo ;
        					owl:maxCardinality 1
     					] ,
     					[ rdf:type owl:Restriction ;
        					owl:onProperty vcard:locality ;
        					owl:maxCardinality 1
     					] ,
     					[ rdf:type owl:Restriction ;
        					owl:onProperty vcard:region ;s
        					owl:maxCardinality 1
     					] ,
     					[ rdf:type owl:Restriction ;
        					owl:onProperty vcard:country-name ;
        					owl:cardinality 1
     					] ;
						rdfs:label "Location"@en ;
						rdfs:comment "vCard definition: 'An object representing a named geographical place'"@en .


###  Respondent
jcpc:Respondent rdfs:subClassOf lkif-action:Agent ,
						[ rdf:type owl:Restriction ;
        					owl:onProperty jcpc:isRespondentOf ;
        					owl:allValuesFrom wikidata:Q329777
     					] ,
     					[ rdf:type owl:Restriction ;
        					owl:onProperty dc:description ;
        					owl:maxCardinality 1
     					] ,
     					[ rdf:type owl:Restriction ;
        					owl:onProperty foaf:name ;
        					owl:cardinality 1
     					] ;
						rdfs:label "Respondent"@en ;
						rdfs:comment "Organisation or person (including those acting under the title of their official role) responding to an Appeal brought to the JCPC"@en .


###  Third Party
jcpc:ThirdParty rdfs:subClassOf lkif-action:Agent ,
						[ rdf:type owl:Restriction ;
        					owl:onProperty jcpc:isThirdPartyOf ;
        					owl:allValuesFrom wikidata:Q329777
     					] ,
     					[ rdf:type owl:Restriction ;
        					owl:onProperty dc:description ;
        					owl:maxCardinality 1
     					] ,
     					[ rdf:type owl:Restriction ;
        					owl:onProperty foaf:name ;
        					owl:cardinality 1
     					] ;
						rdfs:label "Third Party"@en ;
						rdfs:comment "Organisation or person (including those acting under the title of their official role) involved in an Appeal but who is not a party to any contract to which the case relates"@en .


###  Generated by the OWL API (version 4.2.8.20170104-2310) https://github.com/owlcs/owlapi
